compile bundles

src/cddl/pulse/CDDL.Pulse.AST.Bundle.fst
@@ -1,1 +1,531 @@
 module CDDL.Pulse.AST.Bundle
+include CDDL.Pulse.AST.Base
+include CDDL.Pulse.AST.Literal
+include CDDL.Pulse.Bundle.ArrayGroup
+include CDDL.Pulse.Bundle.MapGroup
+include CDDL.Pulse.Bundle.Misc
+open CDDL.Spec.AST.Tactics
+open Pulse.Lib.Pervasives
+open CBOR.Spec.API.Type
+
+module Env = CDDL.Pulse.AST.Env // for validator_env
+module Parse = CDDL.Pulse.AST.Parse // for ancillary_validate_env
+
+let bundle_get_impl_type_steps =
+  delta_attr [
+    `%base_attr;
+    `%bundle_get_impl_type_attr;
+  ] ::
+  delta_only (
+    `%Mkbundle?.b_impl_type ::
+    `%Mkarray_bundle?.ab_impl_type ::
+    `%Mkmap_bundle?.mb_impl_type ::
+    base_delta_only_steps
+  ) ::
+  base_steps
+
+let bundle_steps = 
+  delta_attr [
+    `%base_attr;
+    `%bundle_attr;
+  ] ::
+  delta_only (
+    base_delta_only_steps
+  ) ::
+  base_steps
+
+let bundle_env'
+  (#t: Type0)
+  (vmatch: (perm -> t -> cbor -> slprop))
+  (env: name_env)
+= (n: typ_name env) -> bundle vmatch
+
+let target_spec_env_of_bundle_env
+  (#t: Type0)
+  (#vmatch: (perm -> t -> cbor -> slprop))
+  (se: name_env)
+  (be: bundle_env' vmatch se)
+: Tot (target_spec_env se)
+= fun n -> (be n).b_spec_type
+
+let spec_env_of_bundle_env
+  (#t: Type0)
+  (#vmatch: (perm -> t -> cbor -> slprop))
+  (se: sem_env)
+  (be: bundle_env' vmatch se.se_bound)
+: Pure (spec_env se (target_spec_env_of_bundle_env se.se_bound be))
+    (requires forall n . (Ghost.reveal (be n).b_typ == sem_of_type_sem (se.se_env n)))
+    (ensures fun _ -> True)
+= {
+  tp_spec_typ = fun n -> (be n).b_spec
+}
+
+[@@bundle_attr; sem_attr] // sem_attr for validate_typw
+noeq type bundle_env
+  (#t: Type0)
+  (vmatch: (perm -> t -> cbor -> slprop))
+= {
+  be_ast: wf_ast_env;
+  be_v: Env.validator_env vmatch be_ast.e_sem_env;
+  be_b: bundle_env' vmatch be_ast.e_sem_env.se_bound;
+  be_b_correct: (n: typ_name be_ast.e_sem_env.se_bound) -> Lemma
+    (Ghost.reveal (be_b n).b_typ == sem_of_type_sem (be_ast.e_sem_env.se_env n));
+}
+
+let bundle_env_correct
+  (#t: Type0)
+  (#vmatch: (perm -> t -> cbor -> slprop))
+  (be: bundle_env vmatch)
+  (n: typ_name be.be_ast.e_sem_env.se_bound)
+: Lemma
+  (ensures (Ghost.reveal (be.be_b n).b_typ == sem_of_type_sem (be.be_ast.e_sem_env.se_env n)))
+  [SMTPat (be.be_b n)]
+= be.be_b_correct n
+
+let empty_bundle_env'
+  (#t: Type0)
+  (vmatch: (perm -> t -> cbor -> slprop))
+  (n: typ_name empty_name_env)
+: Tot (bundle vmatch)
+= false_elim ()
+
+let empty_bundle_env'_correct
+  (#t: Type0)
+  (vmatch: (perm -> t -> cbor -> slprop))
+  (n: typ_name empty_name_env)
+: Lemma
+  (Ghost.reveal (empty_bundle_env' vmatch n).b_typ == sem_of_type_sem (empty_sem_env.se_env n))
+= ()
+
+[@@bundle_attr; sem_attr] // sem_attr for validate_typ
+let empty_bundle_env
+  (#t: Type0)
+  (vmatch: (perm -> t -> cbor -> slprop))
+: bundle_env vmatch
+= {
+  be_ast = empty_ast_env;
+  be_v = Env.empty_validator_env _;
+  be_b = empty_bundle_env' _;
+  be_b_correct = empty_bundle_env'_correct vmatch;
+}
+
+let bundle_env_included
+  (#t: Type0)
+  (#vmatch: (perm -> t -> cbor -> slprop))
+  (b1 b2: bundle_env vmatch)
+: Tot prop
+= ast_env_included b1.be_ast b2.be_ast /\
+  (forall (n: typ_name b1.be_ast.e_sem_env.se_bound) .
+    b1.be_b n == b2.be_b n
+  )
+
+let spec_env_of_bundle_env_included
+  (#t: Type0)
+  (#vmatch: (perm -> t -> cbor -> slprop))
+  (b1 b2: bundle_env vmatch)
+: Lemma
+  (requires (bundle_env_included b1 b2))
+  (ensures (spec_env_included (spec_env_of_bundle_env b1.be_ast.e_sem_env b1.be_b) (spec_env_of_bundle_env b2.be_ast.e_sem_env b2.be_b)))
+= ()
+
+[@@bundle_attr]
+let extend_bundle_env'
+  (#t: Type0)
+  (#vmatch: (perm -> t -> cbor -> slprop))
+  (#se: name_env)
+  (be: bundle_env' vmatch se)
+  (n: string { None? (se n) })
+  (b: bundle vmatch)
+: Tot (bundle_env' vmatch (extend_name_env se n NType))
+= fun n' -> if n = n' then b else be n'
+
+let sem_of_typ_sem_wf_ast_env_extend_typ_with_weak
+  (e: wf_ast_env)
+  (new_name: string)
+  (t: typ)
+  (t_wf: ast0_wf_typ t {
+    wf_ast_env_extend_typ_with_weak_pre e new_name t t_wf
+  })
+: Lemma
+  (let e' = (wf_ast_env_extend_typ_with_weak e new_name t t_wf) in
+    sem_of_type_sem (e'.e_sem_env.se_env new_name) == typ_sem e.e_sem_env t
+  )
+= let e' = (wf_ast_env_extend_typ_with_weak e new_name t t_wf) in
+  assert_norm (sem_of_type_sem (e'.e_sem_env.se_env new_name) == typ_sem e.e_sem_env t)
+
+[@@bundle_attr; sem_attr] // sem_attr for validate_typ
+let bundle_env_extend_typ_with_weak
+  (#cbor_t: Type0)
+  (#vmatch: (perm -> cbor_t -> cbor -> slprop))
+  (e: bundle_env vmatch)
+  (new_name: string)
+  (t: typ)
+  (t_wf: ast0_wf_typ t {
+    wf_ast_env_extend_typ_with_weak_pre e.be_ast new_name t t_wf
+  })
+  (w: impl_typ vmatch (typ_sem e.be_ast.e_sem_env t))
+  (p: bundle vmatch {
+    Ghost.reveal p.b_typ == typ_sem e.be_ast.e_sem_env t
+  })
+: Tot (e': bundle_env vmatch {
+      bundle_env_included e e' /\
+      e'.be_ast == wf_ast_env_extend_typ_with_weak e.be_ast new_name t t_wf
+  })
+= {
+    be_ast = wf_ast_env_extend_typ_with_weak e.be_ast new_name t t_wf;
+    be_v = Env.extend_validator_env_with_typ_weak e.be_v new_name () t () w;
+    be_b = extend_bundle_env' e.be_b new_name p;
+    be_b_correct = (fun n' -> if n' = new_name then sem_of_typ_sem_wf_ast_env_extend_typ_with_weak e.be_ast new_name t t_wf else e.be_b_correct n');
+}
+
+[@@bundle_attr; sem_attr] // sem_attr for validate_typ
+let bundle_env_extend_group
+  (#cbor_t: Type0)
+  (#vmatch: (perm -> cbor_t -> cbor -> slprop))
+  (e: bundle_env vmatch)
+  (new_name: string)
+  (t: group)
+  (sq1: squash (e.be_ast.e_sem_env.se_bound new_name == None))
+  (sq2: squash (group_bounded e.be_ast.e_sem_env.se_bound t))
+: Tot (e': bundle_env vmatch {
+      bundle_env_included e e' /\
+      e'.be_ast == wf_ast_env_extend_group e.be_ast new_name t sq1 sq2
+  })
+=
+  {
+    be_ast = wf_ast_env_extend_group e.be_ast new_name t sq1 sq2;
+    be_v = Env.extend_validator_env_with_group e.be_v new_name t () ();
+    be_b = e.be_b;
+    be_b_correct = e.be_b_correct;
+  }
+
+[@@bundle_attr; sem_attr] // sem_attr for ask
+let ancillary_bundle_env
+  (#cbor_t: Type)
+  (vmatch: perm -> cbor_t -> cbor -> slprop)
+  (se: sem_env)
+= (t: typ) -> (t_wf: ast0_wf_typ t {
+      spec_wf_typ se true t t_wf
+  }) -> Pure (option (impl_typ vmatch (typ_sem se t) & bundle vmatch))
+    (requires True)
+    (ensures fun res -> spec_wf_typ se true t t_wf /\
+      begin match res with
+      | None -> True
+      | Some (_, b) -> Ghost.reveal b.b_typ == typ_sem se t
+      end
+    )
+
+[@@sem_attr]
+let ancillary_bundle_env_is_some
+  (#cbor_t: Type)
+  (#vmatch: perm -> cbor_t -> cbor -> slprop)
+  (#se: sem_env)
+  (env: ancillary_bundle_env vmatch se)
+: Tot (Parse.ancillary_parse_env_bool se)
+= fun t t_wf -> Some? (env t t_wf)
+
+[@@bundle_attr; sem_attr] // sem_attr for ask
+let ancillary_bundle_env_extend
+  (#cbor_t: Type)
+  (#vmatch: perm -> cbor_t -> cbor -> slprop)
+  (#se: sem_env)
+  (env1: ancillary_bundle_env vmatch se)
+  (se2: sem_env {
+    sem_env_included se se2
+  })
+: Tot (ancillary_bundle_env vmatch se2)
+= fun t t_wf ->
+  if bounded_wf_typ se.se_bound t t_wf
+  then begin
+    (env1 t t_wf)
+  end
+  else None
+
+[@@bundle_attr; sem_attr] // sem_attr for ask
+let ancillary_bundle_env_set
+  (#cbor_t: Type)
+  (#vmatch: perm -> cbor_t -> cbor -> slprop)
+  (#se: sem_env)
+  (env1: ancillary_bundle_env vmatch se)
+  (t': typ)
+  (t_wf': ast0_wf_typ t' { spec_wf_typ se true t' t_wf' })
+  (v: impl_typ vmatch (typ_sem se t'))
+  (b: bundle vmatch { Ghost.reveal b.b_typ == typ_sem se t' })
+: Tot (ancillary_bundle_env vmatch se)
+= fun t t_wf -> if t = t' && t_wf = t_wf' then Some (v, b) else env1 t t_wf
+
+[@@bundle_attr; sem_attr] // sem_attr for ask
+let ancillary_array_bundle_env
+  (#cbor_t: Type)
+  (cbor_array_iterator_match: perm -> cbor_t -> list cbor -> slprop)
+  (se: sem_env)
+= (t: group) -> (t_wf: ast0_wf_array_group t {
+      spec_wf_array_group se t t_wf
+  }) -> Pure (option (impl_array_group cbor_array_iterator_match (array_group_sem se t) & array_bundle cbor_array_iterator_match))
+    (requires True)
+    (ensures fun res -> spec_wf_array_group se t t_wf /\
+      begin match res with
+      | None -> True
+      | Some (_, b) -> Ghost.reveal b.ab_typ == array_group_sem se t
+      end
+    )
+
+[@@sem_attr]
+let ancillary_array_bundle_env_is_some
+  (#cbor_t: Type)
+  (#cbor_array_iterator_match: perm -> cbor_t -> list cbor -> slprop)
+  (#se: sem_env)
+  (env: ancillary_array_bundle_env cbor_array_iterator_match se)
+: Tot (Parse.ancillary_parse_array_group_env_bool se)
+= fun t t_wf -> Some? (env t t_wf)
+
+[@@bundle_attr; sem_attr] // sem_attr for ask
+let ancillary_array_bundle_env_extend
+  (#cbor_t: Type)
+  (#cbor_array_iterator_match: perm -> cbor_t -> list cbor -> slprop)
+  (#se: sem_env)
+  (env1: ancillary_array_bundle_env cbor_array_iterator_match se)
+  (se2: sem_env {
+    sem_env_included se se2
+  })
+: Tot (ancillary_array_bundle_env cbor_array_iterator_match se2)
+= fun t t_wf ->
+  if bounded_wf_array_group se.se_bound t t_wf
+  then begin
+    (env1 t t_wf)
+  end
+  else None
+
+[@@bundle_attr; sem_attr] // sem_attr for ask
+let ancillary_array_bundle_env_set
+  (#cbor_t: Type)
+  (#cbor_array_iterator_match: perm -> cbor_t -> list cbor -> slprop)
+  (#se: sem_env)
+  (env1: ancillary_array_bundle_env cbor_array_iterator_match se)
+  (t': group)
+  (t_wf': ast0_wf_array_group t' { spec_wf_array_group se t' t_wf' })
+  (v: impl_array_group cbor_array_iterator_match (array_group_sem se t'))
+  (b: array_bundle cbor_array_iterator_match { Ghost.reveal b.ab_typ == array_group_sem se t' })
+: Tot (ancillary_array_bundle_env cbor_array_iterator_match se)
+= fun t t_wf -> if t = t' && t_wf = t_wf' then Some (v, b) else env1 t t_wf
+
+module U64 = FStar.UInt64
+module U8 = FStar.UInt8
+module I64 = FStar.Int64
+module V = CDDL.Pulse.AST.Validate
+module SZ = FStar.SizeT
+open CBOR.Pulse.API.Base
+
+[@@bundle_attr]
+let impl_bundle_elem_type
+  (#ty: Type0)
+  (vmatch: (perm -> ty -> cbor -> slprop))
+  (cbor_get_major_type: get_major_type_t vmatch)
+  (cbor_destr_int64: read_uint64_t vmatch)
+  (cbor_get_string: get_string_t vmatch)
+  (cbor_destr_simple: read_simple_value_t vmatch)
+  (l: elem_typ)
+: Pure (bundle vmatch)
+    (requires wf_elem_typ l)
+    (ensures fun res ->
+      wf_elem_typ l /\
+      Ghost.reveal res.b_typ == elem_typ_sem l
+    )
+= match l with
+  | ELiteral l -> bundle_unit _ (spec_literal (eval_literal l))
+  | EBool -> bundle_bool cbor_destr_simple
+  | ESimple -> bundle_simple cbor_destr_simple
+  | EByteString -> bundle_bytes cbor_get_string
+  | ETextString -> bundle_text cbor_get_string
+  | EUInt -> bundle_uint cbor_destr_int64
+  | ENInt -> bundle_nint cbor_destr_int64
+  | EAlwaysFalse -> bundle_always_false _ (spec_always_false (fun _ -> true))
+  | EAny -> bundle_any _
+
+#push-options "--z3rlimit 1024 --query_stats --ifuel 4 --fuel 4 --split_queries always"
+
+[@@bundle_attr]
+let rec impl_bundle_wf_type
+  (#cbor_t #t2 #t_arr #t_map: Type0)
+  (#vmatch: (perm -> cbor_t -> cbor -> slprop))
+  (#vmatch2: (perm -> t2 -> (cbor & cbor) -> slprop))
+  (#cbor_array_iterator_match: (perm -> t_arr -> list cbor -> slprop))
+  (#cbor_map_iterator_match: (perm -> t_map -> list (cbor & cbor) -> slprop))
+  (impl: cbor_impl vmatch vmatch2 cbor_array_iterator_match cbor_map_iterator_match)
+  (env: bundle_env vmatch)
+  (ancillary_v: Parse.ancillary_validate_env vmatch env.be_ast.e_sem_env)
+  (ancillary: ancillary_bundle_env vmatch env.be_ast.e_sem_env)
+  (ancillary_ag: ancillary_array_bundle_env cbor_array_iterator_match env.be_ast.e_sem_env)
+  (#t: typ)
+  (t_wf: ast0_wf_typ t)
+: Pure (bundle vmatch)
+    (requires 
+    spec_wf_typ env.be_ast.e_sem_env true t t_wf /\ SZ.fits_u64
+    /\ None? (Parse.ask_zero_copy_wf_type (Parse.ancillary_validate_env_is_some ancillary_v) (ancillary_bundle_env_is_some ancillary) (ancillary_array_bundle_env_is_some ancillary_ag) t_wf)
+    )
+    (ensures fun res ->
+      spec_wf_typ env.be_ast.e_sem_env true t t_wf /\
+      Ghost.reveal res.b_typ == typ_sem env.be_ast.e_sem_env t
+    )
+    (decreases t_wf)
+= match t_wf with
+  | WfTRewrite _ _ s ->
+    bundle_type_ext (impl_bundle_wf_type impl env ancillary_v ancillary ancillary_ag s) (typ_sem env.be_ast.e_sem_env t) ()
+  | WfTTagged tg _ s ->
+    let p = impl_bundle_wf_type impl env ancillary_v ancillary ancillary_ag s in
+    begin match tg with
+    | None -> bundle_tagged_none impl.cbor_get_tagged_tag impl.cbor_get_tagged_payload p
+    | Some tag -> bundle_tagged_some impl.cbor_get_tagged_payload (U64.uint_to_t tag) p
+    end
+  | WfTChoice _ _ s1 s2 ->
+    let p1 = impl_bundle_wf_type impl env ancillary_v ancillary ancillary_ag s1 in
+    let p2 = impl_bundle_wf_type impl env ancillary_v ancillary ancillary_ag s2 in
+    (bundle_choice p1 (V.validate_typ impl env.be_v true _ s1) p2 ())
+  | WfTElem e -> (impl_bundle_elem_type vmatch impl.cbor_get_major_type impl.cbor_destr_int64 impl.cbor_get_string impl.cbor_destr_simple e)
+  | WfTDetCbor _ _ s ->
+    let p = impl_bundle_wf_type impl env ancillary_v ancillary ancillary_ag s in
+    bundle_type_ext
+      (bundle_det_cbor impl.cbor_get_string impl.cbor_det_parse p)
+      (typ_sem env.be_ast.e_sem_env t) ()
+  | WfTStrSize k base range lo hi ->
+    bundle_type_ext
+      (bundle_str_size impl.cbor_get_string (U8.uint_to_t k) (U64.uint_to_t lo) (U64.uint_to_t hi))
+      (typ_sem env.be_ast.e_sem_env t) ()
+  | WfTIntRange _ _ _ lo hi ->
+    if hi < 0
+    then (bundle_int_range_neg_int64 impl.cbor_destr_int64 (U64.uint_to_t ((-1) - lo)) (U64.uint_to_t ((-1) - hi)))
+    else if lo >= 0
+    then (bundle_int_range_uint64 impl.cbor_destr_int64 (U64.uint_to_t lo) (U64.uint_to_t hi))
+    else (bundle_int_range_int64 impl.cbor_get_major_type impl.cbor_destr_int64 (I64.int_to_t lo) (I64.int_to_t hi))
+  | WfTDef n -> env.be_b n
+  | WfTArray _ s ->
+    let ps = impl_bundle_wf_array_group impl env ancillary_v ancillary ancillary_ag s in
+    (bundle_array impl.cbor_array_iterator_init ps)
+  | WfTMap _ _ s ->
+    let ps = impl_bundle_wf_map_group impl env ancillary_v ancillary ancillary_ag s in
+    (bundle_map ps)
+
+and impl_bundle_wf_array_group
+  (#cbor_t #t2 #t_arr #t_map: Type0)
+  (#vmatch: (perm -> cbor_t -> cbor -> slprop))
+  (#vmatch2: (perm -> t2 -> (cbor & cbor) -> slprop))
+  (#cbor_array_iterator_match: (perm -> t_arr -> list cbor -> slprop))
+  (#cbor_map_iterator_match: (perm -> t_map -> list (cbor & cbor) -> slprop))
+  (impl: cbor_impl vmatch vmatch2 cbor_array_iterator_match cbor_map_iterator_match)
+  (env: bundle_env vmatch)
+  (ancillary_v: Parse.ancillary_validate_env vmatch env.be_ast.e_sem_env)
+  (ancillary: ancillary_bundle_env vmatch env.be_ast.e_sem_env)
+  (ancillary_ag: ancillary_array_bundle_env cbor_array_iterator_match env.be_ast.e_sem_env)
+  (#t: group)
+  (t_wf: ast0_wf_array_group t)
+: Pure (array_bundle cbor_array_iterator_match)
+    (requires 
+    spec_wf_array_group env.be_ast.e_sem_env t t_wf /\ SZ.fits_u64
+    /\ None? (Parse.ask_zero_copy_wf_array_group (Parse.ancillary_validate_env_is_some ancillary_v) (ancillary_bundle_env_is_some ancillary) (ancillary_array_bundle_env_is_some ancillary_ag) t_wf)
+    )
+    (ensures fun res ->
+      spec_wf_array_group env.be_ast.e_sem_env t t_wf /\
+      Ghost.reveal res.ab_typ == array_group_sem env.be_ast.e_sem_env t
+    )
+    (decreases t_wf)
+= match t_wf with
+  | WfAElem _ _ _ t_wf' ->
+    let pt = impl_bundle_wf_type impl env ancillary_v ancillary ancillary_ag t_wf' in
+    (bundle_array_group_item impl.cbor_array_iterator_next pt)
+  | WfAZeroOrOne _ t_wf' ->
+    let pe = impl_bundle_wf_array_group impl env ancillary_v ancillary ancillary_ag t_wf' in
+    (bundle_array_group_zero_or_one pe (V.validate_array_group impl env.be_v _ t_wf') ())
+  | WfAZeroOrOneOrMore _ t_wf' g' ->
+    // HERE I need function pointers, so I MUST NOT do a recursive call
+    let Some (ve, be) = ancillary_ag _ t_wf' in
+      begin match g' with
+      | GZeroOrMore _ ->
+        (bundle_array_group_zero_or_more impl.cbor_array_iterator_share impl.cbor_array_iterator_gather be ve ())
+      | _ ->
+        (bundle_array_group_one_or_more impl.cbor_array_iterator_share impl.cbor_array_iterator_gather be ve ())
+      end
+  | WfAConcat _ _ t_wf1 t_wf2 ->
+    let pg1 = impl_bundle_wf_array_group impl env ancillary_v ancillary ancillary_ag t_wf1 in
+    let pg2 = impl_bundle_wf_array_group impl env ancillary_v ancillary ancillary_ag t_wf2 in
+    (bundle_array_group_concat impl.cbor_array_iterator_length impl.cbor_array_iterator_share impl.cbor_array_iterator_gather impl.cbor_array_iterator_truncate pg1 (V.validate_array_group impl env.be_v _ t_wf1) pg2 ())
+  | WfAChoice _ _ t_wf1 t_wf2 ->
+    let pg1 = impl_bundle_wf_array_group impl env ancillary_v ancillary ancillary_ag t_wf1 in
+    let pg2 = impl_bundle_wf_array_group impl env ancillary_v ancillary ancillary_ag t_wf2 in
+    (bundle_array_group_choice pg1 (V.validate_array_group impl env.be_v _ t_wf1) pg2 ())
+  | WfARewrite _ _ t_wf2 ->
+    bundle_array_group_ext'
+      (impl_bundle_wf_array_group impl env ancillary_v ancillary ancillary_ag t_wf2)
+      (array_group_sem env.be_ast.e_sem_env t) ()
+
+and impl_bundle_wf_map_group
+  (#cbor_t #t2 #t_arr #t_map: Type0)
+  (#vmatch: (perm -> cbor_t -> cbor -> slprop))
+  (#vmatch2: (perm -> t2 -> (cbor & cbor) -> slprop))
+  (#cbor_array_iterator_match: (perm -> t_arr -> list cbor -> slprop))
+  (#cbor_map_iterator_match: (perm -> t_map -> list (cbor & cbor) -> slprop))
+  (impl: cbor_impl vmatch vmatch2 cbor_array_iterator_match cbor_map_iterator_match)
+  (env: bundle_env vmatch)
+  (ancillary_v: Parse.ancillary_validate_env vmatch env.be_ast.e_sem_env)
+  (ancillary: ancillary_bundle_env vmatch env.be_ast.e_sem_env)
+  (ancillary_ag: ancillary_array_bundle_env cbor_array_iterator_match env.be_ast.e_sem_env)
+  (#t: elab_map_group)
+  (t_wf: ast0_wf_parse_map_group t)
+: Pure (map_bundle vmatch)
+    (requires 
+    spec_wf_parse_map_group env.be_ast.e_sem_env t t_wf /\ SZ.fits_u64
+    /\ None? (Parse.ask_zero_copy_wf_map_group (Parse.ancillary_validate_env_is_some ancillary_v) (ancillary_bundle_env_is_some ancillary) (ancillary_array_bundle_env_is_some ancillary_ag) t_wf)
+    )
+    (ensures fun res ->
+      spec_wf_parse_map_group env.be_ast.e_sem_env t t_wf /\
+      Ghost.reveal res.mb_typ == elab_map_group_sem env.be_ast.e_sem_env t /\
+      res.mb_footprint == spec_map_group_footprint env.be_ast.e_sem_env t
+    )
+    (decreases t_wf)
+= match t_wf with
+  | WfMChoice _ s1 _ s2 ->
+    let ps1 = impl_bundle_wf_map_group impl env ancillary_v ancillary ancillary_ag s1 in
+    let ps2 = impl_bundle_wf_map_group impl env ancillary_v ancillary ancillary_ag s2 in
+    (bundle_map_choice ps1 (V.validate_map_group impl env.be_v _ s1) ps2 ())
+  | WfMConcat _ s1 _ s2 ->
+    let ps1 = impl_bundle_wf_map_group impl env ancillary_v ancillary ancillary_ag s1 in
+    let ps2 = impl_bundle_wf_map_group impl env ancillary_v ancillary ancillary_ag s2 in
+    (bundle_map_concat impl.cbor_share impl.cbor_gather ps1 ps2 ())
+  | WfMZeroOrOne _ s1 ->
+    let ps1 = impl_bundle_wf_map_group impl env ancillary_v ancillary ancillary_ag s1 in
+    bundle_map_ext'
+      (bundle_map_zero_or_one
+        ps1
+        (V.validate_map_group impl env.be_v _ s1)
+        ()
+      )
+      (t_choice ps1.mb_footprint t_always_false)
+      ()
+  | WfMLiteral cut key _ s ->
+    let ps1 = impl_bundle_wf_type impl env ancillary_v ancillary ancillary_ag s in
+        (bundle_map_match_item_for
+          impl.cbor_map_get
+          (with_literal
+            impl.cbor_mk_int64
+            impl.cbor_elim_int64
+            impl.cbor_mk_simple
+            impl.cbor_elim_simple
+            impl.cbor_mk_string
+            key
+          )
+          cut
+          ps1
+        )
+  | WfMZeroOrMore _ key_except _ s_key s_key_except s_value ->
+    let Some (v_key, p_key) = ancillary _ s_key in
+    let Some (v_key_except) = ancillary_v key_except in
+    let Some (v_value, p_value) = ancillary _ s_value in
+            (bundle_map_zero_or_more
+              impl.cbor_map_iterator_init
+              impl.cbor_map_iterator_share
+              impl.cbor_map_iterator_gather
+              p_key
+              v_key
+              v_key_except
+              p_value
+              v_value
+            )
